IIO: fix <=, fill some proofs
This previously stated GetTraceActions <= IOActions.

io/IIO.fst
@@ -75,12 +75,56 @@ let (<=) (flag1:tflag) (flag2:tflag) =
   match flag1, flag2 with
   | NoActions, _ -> True
   | GetTraceActions, NoActions -> False
+  | GetTraceActions, IOActions -> False
   | GetTraceActions, _ -> True
   | IOActions, NoActions -> False
   | IOActions, GetTraceActions -> False
   | IOActions, _ -> True
   | AllActions, AllActions -> True
   | AllActions, _ -> False
+
+let plus_compat_le (f1 f2 : tflag) : Lemma (f1 <= f1+f2) = ()
+let plus_comm      (f1 f2 : tflag) : Lemma (f1+f2 == f2+f1) = ()
+
+let rec sat_le (f1:tflag) (f2:tflag{f1 <= f2}) (m : iio 'a) :
+  Lemma (satisfies m f1 ==> satisfies m f2) =
+  match m with
+  | Return _ -> ()
+  | PartialCall i o ->
+    Classical.forall_intro
+     ((fun r -> sat_le f1 f2 (o r)) <: r:_ -> Lemma (satisfies (o r) f1 ==> satisfies (o r) f2))
+  | Call _ f i o ->
+    Classical.forall_intro
+     ((fun r -> sat_le f1 f2 (o r)) <: r:_ -> Lemma (satisfies (o r) f1 ==> satisfies (o r) f2))
+
+let rec sat_bind (fl:tflag) (v : iio 'a) (f : 'a -> iio 'b)
+  : Lemma (v `satisfies` fl /\ (forall x. f x `satisfies` fl) ==> free_bind _ _ _ _ v f `satisfies` fl)
+  =
+  match v with
+  | Return _ -> ()
+  | PartialCall i o ->
+  Classical.forall_intro
+   ((fun r -> sat_bind fl (o r) f) <: r:_ -> Lemma ((o r) `satisfies` fl /\ (forall x. f x `satisfies` fl) ==> free_bind _ _ _ _ (o r) f `satisfies` fl))
+
+  | Call _ _ i o ->
+  Classical.forall_intro
+   ((fun r -> sat_bind fl (o r) f) <: r:_ -> Lemma ((o r) `satisfies` fl /\ (forall x. f x `satisfies` fl) ==> free_bind _ _ _ _ (o r) f `satisfies` fl))
+
+let dm_iio_bind_is_free_bind a b wp_v wp_f v f
+: Lemma (dm_iio_bind a b wp_v wp_f v f == free_bind _ _ _ _ v f)
+=
+  let r = dm_iio_bind a b wp_v wp_f v f in
+  assert (r == free_bind _ _ _ _ v f)
+
+let sat_bind_add (fl_v fl_f:tflag) (v : iio 'a) (f : 'a -> iio 'b)
+  : Lemma (v `satisfies` fl_v /\ (forall x. f x `satisfies` fl_f) ==> free_bind _ _ _ _ v f `satisfies` (fl_v + fl_f))
+  =
+  sat_le fl_v (fl_v + fl_f) v;
+  let aux x : Lemma (f x `satisfies` fl_f ==> f x `satisfies` (fl_v + fl_f)) =
+    sat_le fl_f (fl_v + fl_f) (f x)
+  in
+  Classical.forall_intro aux;
+  sat_bind (fl_v + fl_f) v f
 
 (** ** Defining F* Effect **)
 
@@ -95,31 +139,35 @@ val dm_giio_bind  :
   a: Type ->
   b: Type ->
   flag_v : erased tflag ->
-  flag_f : erased tflag ->
   wp_v: Hist.hist a ->
-  wp_f: (_: a -> Hist.hist b) ->
+  flag_f : erased tflag ->
+  wp_f: (a -> Hist.hist b) ->
   v: dm_giio a flag_v wp_v ->
   f: (x: a -> dm_giio b flag_f (wp_f x)) ->
   Tot (dm_giio b (flag_v + flag_f) (hist_bind wp_v wp_f))
-let dm_giio_bind a b flag_v flag_f wp_v wp_f v f : (dm_giio b (flag_v + flag_f) (hist_bind wp_v wp_f)) = 
+let dm_giio_bind a b flag_v wp_v flag_f wp_f v f : (dm_giio b (flag_v + flag_f) (hist_bind wp_v wp_f)) =
   let r = dm_iio_bind a b wp_v wp_f v f in
-  assume (v `satisfies` flag_v /\ (forall x. f x `satisfies` flag_f) ==> r `satisfies` (flag_v + flag_f));
+  sat_bind_add flag_v flag_f v f;
+  dm_iio_bind_is_free_bind a b wp_v wp_f v f;
+  assert (free_bind _ _ _ _ v f `satisfies` (flag_v + flag_f));
   r
 
 val dm_giio_subcomp : 
   a: Type ->
   flag1 : erased tflag ->
-  flag2 : erased tflag ->
   wp1: hist a ->
+  flag2 : erased tflag ->
   wp2: hist a ->
   f: dm_giio a flag1 wp1 ->
   Pure (dm_giio a flag2 wp2) ((flag1 <= flag2) /\ hist_ord wp2 wp1) (fun _ -> True)
-let dm_giio_subcomp a flag1 flag2 wp1 wp2 f = 
-  admit ();
+let dm_giio_subcomp a flag1 wp1 flag2 wp2 f =
+  sat_le flag1 flag2 f;
   dm_iio_subcomp a wp1 wp2 f
 
-let dm_giio_if_then_else (a : Type u#a) (fl1 fl2:erased tflag)
-  (wp1 wp2: hist a) (f : dm_giio a fl1 wp1) (g : dm_giio a fl2 wp2) (b : bool) : Type =
+let dm_giio_if_then_else (a : Type u#a)
+  (fl1 : erased tflag) (wp1 : hist a)
+  (fl2 : erased tflag) (wp2 : hist a)
+  (f : dm_giio a fl1 wp1) (g : dm_giio a fl2 wp2) (b : bool) : Type =
   dm_giio a (fl1 + fl2) (hist_if_then_else wp1 wp2 b)
 
 total
@@ -149,8 +197,8 @@ let lift_pure_dm_giio a w f =
   FStar.Monotonic.Pure.elim_pure_wp_monotonicity_forall ();
   let lhs : dm_giio _ NoActions _ = dm_giio_partial_return (as_requires w) in
   let rhs = (fun (pre:(squash (as_requires w))) -> dm_giio_return a (f pre)) in
-  let m = dm_giio_bind _ _ NoActions NoActions _ _ lhs rhs in
-  dm_giio_subcomp a NoActions NoActions _ _ m
+  let m = dm_giio_bind _ _ NoActions _ NoActions _ lhs rhs in
+  dm_giio_subcomp a NoActions _ NoActions _ m
   
 sub_effect PURE ~> IIOwp = lift_pure_dm_giio
 
@@ -179,7 +227,9 @@ let get_trace (isTrusted:bool) : IIOwp trace GetTraceActions
 // val ctx_s : (fl:erased tflag) -> IIO unit fl (fun _ -> True) (fun _ _ _ -> True) 
 
 private
-let performance_test (#fl:tflag) : IIOwp unit (fl+IOActions) (fun p h -> forall lt. (List.length lt == 6) \/ (List.length lt == 7) ==> p lt ()) =
+let performance_test (#fl:tflag) : IIOwp unit (fl+IOActions) (fun p h -> forall lt. (List.length lt == 6) \/ (List.length lt == 7) ==> p lt ())
+  by (compute ())
+=
   let fd = static_cmd true Openfile "../Makefile" in
   let fd = static_cmd true Openfile "../Makefile" in
   let fd = static_cmd true Openfile "../Makefile" in
